src/Actions/MappingEnumerator.dfy
@@ -53,11 +53,6 @@ module Mapped {
       assert ValidWrappedProduced(consumed, produced, wrapped.produced);
     }
 
-    ghost predicate CanConsume(consumed: seq<()>, produced: seq<Option<R>>, next: ())
-      decreases height
-    {
-      true
-    }
     ghost predicate CanProduce(consumed: seq<()>, produced: seq<Option<R>>)
       decreases height
     {
@@ -71,7 +66,7 @@ module Mapped {
 
     method Invoke(t: ()) returns (r: Option<R>) 
       requires Valid()
-      requires CanConsume(consumed, produced, t)
+      requires exists r :: CanProduce(consumed + [t], produced + [r])
       modifies Repr
       decreases height
       ensures Valid()
